new/code/math.v
@@ -6,6 +6,9 @@ Section code.
 Context `{ffi_syntax}.
 
 
+(* 9223372036854775807 *)
+Definition MaxInt64 : Z := 9223372036854775808 - 1.
+
 (* 18446744073709551615 *)
 Definition MaxUint64 : Z := 18446744073709551616 - 1.
 
