new/generatedproof/go_etcd_io/etcd/api/v3/etcdserverpb.v
@@ -4,6 +4,280 @@ From New.golang Require Import theory.
 
 Axiom falso : False.
 
+Module Compare_CompareResult.
+Section def.
+Context `{ffi_syntax}.
+Definition t := w32.
+End def.
+End Compare_CompareResult.
+Module Compare_CompareTarget.
+Section def.
+Context `{ffi_syntax}.
+Definition t := w32.
+End def.
+End Compare_CompareTarget.
+Module ResponseHeader.
+Section def.
+Context `{ffi_syntax}.
+Record t := mk {
+  ClusterId' : w64;
+  MemberId' : w64;
+  Revision' : w64;
+  RaftTerm' : w64;
+  XXX_NoUnkeyedLiteral' : unit;
+  XXX_unrecognized' : slice.t;
+  XXX_sizecache' : w32;
+}.
+End def.
+End ResponseHeader.
+
+
+Global Instance settable_ResponseHeader `{ffi_syntax}: Settable _ :=
+  settable! ResponseHeader.mk < ResponseHeader.ClusterId'; ResponseHeader.MemberId'; ResponseHeader.Revision'; ResponseHeader.RaftTerm'; ResponseHeader.XXX_NoUnkeyedLiteral'; ResponseHeader.XXX_unrecognized'; ResponseHeader.XXX_sizecache' >.
+Global Instance into_val_ResponseHeader `{ffi_syntax} : IntoVal ResponseHeader.t.
+Admitted.
+
+Global Instance into_val_typed_ResponseHeader `{ffi_syntax} : IntoValTyped ResponseHeader.t etcdserverpb.ResponseHeader :=
+{|
+  default_val := ResponseHeader.mk (default_val _) (default_val _) (default_val _) (default_val _) (default_val _) (default_val _) (default_val _);
+  to_val_has_go_type := ltac:(destruct falso);
+  default_val_eq_zero_val := ltac:(destruct falso);
+  to_val_inj := ltac:(destruct falso);
+  to_val_eqdec := ltac:(solve_decision);
+|}.
+Global Instance into_val_struct_field_ResponseHeader_ClusterId `{ffi_syntax} : IntoValStructField "ClusterId" etcdserverpb.ResponseHeader ResponseHeader.ClusterId'.
+Admitted.
+
+Global Instance into_val_struct_field_ResponseHeader_MemberId `{ffi_syntax} : IntoValStructField "MemberId" etcdserverpb.ResponseHeader ResponseHeader.MemberId'.
+Admitted.
+
+Global Instance into_val_struct_field_ResponseHeader_Revision `{ffi_syntax} : IntoValStructField "Revision" etcdserverpb.ResponseHeader ResponseHeader.Revision'.
+Admitted.
+
+Global Instance into_val_struct_field_ResponseHeader_RaftTerm `{ffi_syntax} : IntoValStructField "RaftTerm" etcdserverpb.ResponseHeader ResponseHeader.RaftTerm'.
+Admitted.
+
+Global Instance into_val_struct_field_ResponseHeader_XXX_NoUnkeyedLiteral `{ffi_syntax} : IntoValStructField "XXX_NoUnkeyedLiteral" etcdserverpb.ResponseHeader ResponseHeader.XXX_NoUnkeyedLiteral'.
+Admitted.
+
+Global Instance into_val_struct_field_ResponseHeader_XXX_unrecognized `{ffi_syntax} : IntoValStructField "XXX_unrecognized" etcdserverpb.ResponseHeader ResponseHeader.XXX_unrecognized'.
+Admitted.
+
+Global Instance into_val_struct_field_ResponseHeader_XXX_sizecache `{ffi_syntax} : IntoValStructField "XXX_sizecache" etcdserverpb.ResponseHeader ResponseHeader.XXX_sizecache'.
+Admitted.
+
+Instance wp_struct_make_ResponseHeader `{ffi_semantics} `{!ffi_interp ffi} `{!heapGS Σ} ClusterId' MemberId' Revision' RaftTerm' XXX_NoUnkeyedLiteral' XXX_unrecognized' XXX_sizecache':
+  PureWp True
+    (struct.make etcdserverpb.ResponseHeader (alist_val [
+      "ClusterId" ::= #ClusterId';
+      "MemberId" ::= #MemberId';
+      "Revision" ::= #Revision';
+      "RaftTerm" ::= #RaftTerm';
+      "XXX_NoUnkeyedLiteral" ::= #XXX_NoUnkeyedLiteral';
+      "XXX_unrecognized" ::= #XXX_unrecognized';
+      "XXX_sizecache" ::= #XXX_sizecache'
+    ]))%V
+    #(ResponseHeader.mk ClusterId' MemberId' Revision' RaftTerm' XXX_NoUnkeyedLiteral' XXX_unrecognized' XXX_sizecache').
+Admitted.
+
+Module RangeResponse.
+Section def.
+Context `{ffi_syntax}.
+Record t := mk {
+  Header' : loc;
+  Kvs' : slice.t;
+  More' : bool;
+  Count' : w64;
+  XXX_NoUnkeyedLiteral' : unit;
+  XXX_unrecognized' : slice.t;
+  XXX_sizecache' : w32;
+}.
+End def.
+End RangeResponse.
+
+
+Global Instance settable_RangeResponse `{ffi_syntax}: Settable _ :=
+  settable! RangeResponse.mk < RangeResponse.Header'; RangeResponse.Kvs'; RangeResponse.More'; RangeResponse.Count'; RangeResponse.XXX_NoUnkeyedLiteral'; RangeResponse.XXX_unrecognized'; RangeResponse.XXX_sizecache' >.
+Global Instance into_val_RangeResponse `{ffi_syntax} : IntoVal RangeResponse.t.
+Admitted.
+
+Global Instance into_val_typed_RangeResponse `{ffi_syntax} : IntoValTyped RangeResponse.t etcdserverpb.RangeResponse :=
+{|
+  default_val := RangeResponse.mk (default_val _) (default_val _) (default_val _) (default_val _) (default_val _) (default_val _) (default_val _);
+  to_val_has_go_type := ltac:(destruct falso);
+  default_val_eq_zero_val := ltac:(destruct falso);
+  to_val_inj := ltac:(destruct falso);
+  to_val_eqdec := ltac:(solve_decision);
+|}.
+Global Instance into_val_struct_field_RangeResponse_Header `{ffi_syntax} : IntoValStructField "Header" etcdserverpb.RangeResponse RangeResponse.Header'.
+Admitted.
+
+Global Instance into_val_struct_field_RangeResponse_Kvs `{ffi_syntax} : IntoValStructField "Kvs" etcdserverpb.RangeResponse RangeResponse.Kvs'.
+Admitted.
+
+Global Instance into_val_struct_field_RangeResponse_More `{ffi_syntax} : IntoValStructField "More" etcdserverpb.RangeResponse RangeResponse.More'.
+Admitted.
+
+Global Instance into_val_struct_field_RangeResponse_Count `{ffi_syntax} : IntoValStructField "Count" etcdserverpb.RangeResponse RangeResponse.Count'.
+Admitted.
+
+Global Instance into_val_struct_field_RangeResponse_XXX_NoUnkeyedLiteral `{ffi_syntax} : IntoValStructField "XXX_NoUnkeyedLiteral" etcdserverpb.RangeResponse RangeResponse.XXX_NoUnkeyedLiteral'.
+Admitted.
+
+Global Instance into_val_struct_field_RangeResponse_XXX_unrecognized `{ffi_syntax} : IntoValStructField "XXX_unrecognized" etcdserverpb.RangeResponse RangeResponse.XXX_unrecognized'.
+Admitted.
+
+Global Instance into_val_struct_field_RangeResponse_XXX_sizecache `{ffi_syntax} : IntoValStructField "XXX_sizecache" etcdserverpb.RangeResponse RangeResponse.XXX_sizecache'.
+Admitted.
+
+Instance wp_struct_make_RangeResponse `{ffi_semantics} `{!ffi_interp ffi} `{!heapGS Σ} Header' Kvs' More' Count' XXX_NoUnkeyedLiteral' XXX_unrecognized' XXX_sizecache':
+  PureWp True
+    (struct.make etcdserverpb.RangeResponse (alist_val [
+      "Header" ::= #Header';
+      "Kvs" ::= #Kvs';
+      "More" ::= #More';
+      "Count" ::= #Count';
+      "XXX_NoUnkeyedLiteral" ::= #XXX_NoUnkeyedLiteral';
+      "XXX_unrecognized" ::= #XXX_unrecognized';
+      "XXX_sizecache" ::= #XXX_sizecache'
+    ]))%V
+    #(RangeResponse.mk Header' Kvs' More' Count' XXX_NoUnkeyedLiteral' XXX_unrecognized' XXX_sizecache').
+Admitted.
+
+Module Compare.
+Section def.
+Context `{ffi_syntax}.
+Record t := mk {
+  Result' : w32;
+  Target' : w32;
+  Key' : slice.t;
+  TargetUnion' : interface.t;
+  RangeEnd' : slice.t;
+  XXX_NoUnkeyedLiteral' : unit;
+  XXX_unrecognized' : slice.t;
+  XXX_sizecache' : w32;
+}.
+End def.
+End Compare.
+
+
+Global Instance settable_Compare `{ffi_syntax}: Settable _ :=
+  settable! Compare.mk < Compare.Result'; Compare.Target'; Compare.Key'; Compare.TargetUnion'; Compare.RangeEnd'; Compare.XXX_NoUnkeyedLiteral'; Compare.XXX_unrecognized'; Compare.XXX_sizecache' >.
+Global Instance into_val_Compare `{ffi_syntax} : IntoVal Compare.t.
+Admitted.
+
+Global Instance into_val_typed_Compare `{ffi_syntax} : IntoValTyped Compare.t etcdserverpb.Compare :=
+{|
+  default_val := Compare.mk (default_val _) (default_val _) (default_val _) (default_val _) (default_val _) (default_val _) (default_val _) (default_val _);
+  to_val_has_go_type := ltac:(destruct falso);
+  default_val_eq_zero_val := ltac:(destruct falso);
+  to_val_inj := ltac:(destruct falso);
+  to_val_eqdec := ltac:(solve_decision);
+|}.
+Global Instance into_val_struct_field_Compare_Result `{ffi_syntax} : IntoValStructField "Result" etcdserverpb.Compare Compare.Result'.
+Admitted.
+
+Global Instance into_val_struct_field_Compare_Target `{ffi_syntax} : IntoValStructField "Target" etcdserverpb.Compare Compare.Target'.
+Admitted.
+
+Global Instance into_val_struct_field_Compare_Key `{ffi_syntax} : IntoValStructField "Key" etcdserverpb.Compare Compare.Key'.
+Admitted.
+
+Global Instance into_val_struct_field_Compare_TargetUnion `{ffi_syntax} : IntoValStructField "TargetUnion" etcdserverpb.Compare Compare.TargetUnion'.
+Admitted.
+
+Global Instance into_val_struct_field_Compare_RangeEnd `{ffi_syntax} : IntoValStructField "RangeEnd" etcdserverpb.Compare Compare.RangeEnd'.
+Admitted.
+
+Global Instance into_val_struct_field_Compare_XXX_NoUnkeyedLiteral `{ffi_syntax} : IntoValStructField "XXX_NoUnkeyedLiteral" etcdserverpb.Compare Compare.XXX_NoUnkeyedLiteral'.
+Admitted.
+
+Global Instance into_val_struct_field_Compare_XXX_unrecognized `{ffi_syntax} : IntoValStructField "XXX_unrecognized" etcdserverpb.Compare Compare.XXX_unrecognized'.
+Admitted.
+
+Global Instance into_val_struct_field_Compare_XXX_sizecache `{ffi_syntax} : IntoValStructField "XXX_sizecache" etcdserverpb.Compare Compare.XXX_sizecache'.
+Admitted.
+
+Instance wp_struct_make_Compare `{ffi_semantics} `{!ffi_interp ffi} `{!heapGS Σ} Result' Target' Key' TargetUnion' RangeEnd' XXX_NoUnkeyedLiteral' XXX_unrecognized' XXX_sizecache':
+  PureWp True
+    (struct.make etcdserverpb.Compare (alist_val [
+      "Result" ::= #Result';
+      "Target" ::= #Target';
+      "Key" ::= #Key';
+      "TargetUnion" ::= #TargetUnion';
+      "RangeEnd" ::= #RangeEnd';
+      "XXX_NoUnkeyedLiteral" ::= #XXX_NoUnkeyedLiteral';
+      "XXX_unrecognized" ::= #XXX_unrecognized';
+      "XXX_sizecache" ::= #XXX_sizecache'
+    ]))%V
+    #(Compare.mk Result' Target' Key' TargetUnion' RangeEnd' XXX_NoUnkeyedLiteral' XXX_unrecognized' XXX_sizecache').
+Admitted.
+
+Module isCompare_TargetUnion.
+Section def.
+Context `{ffi_syntax}.
+Definition t := interface.t.
+End def.
+End isCompare_TargetUnion.
+Module TxnResponse.
+Section def.
+Context `{ffi_syntax}.
+Record t := mk {
+  Header' : loc;
+  Succeeded' : bool;
+  Responses' : slice.t;
+  XXX_NoUnkeyedLiteral' : unit;
+  XXX_unrecognized' : slice.t;
+  XXX_sizecache' : w32;
+}.
+End def.
+End TxnResponse.
+
+
+Global Instance settable_TxnResponse `{ffi_syntax}: Settable _ :=
+  settable! TxnResponse.mk < TxnResponse.Header'; TxnResponse.Succeeded'; TxnResponse.Responses'; TxnResponse.XXX_NoUnkeyedLiteral'; TxnResponse.XXX_unrecognized'; TxnResponse.XXX_sizecache' >.
+Global Instance into_val_TxnResponse `{ffi_syntax} : IntoVal TxnResponse.t.
+Admitted.
+
+Global Instance into_val_typed_TxnResponse `{ffi_syntax} : IntoValTyped TxnResponse.t etcdserverpb.TxnResponse :=
+{|
+  default_val := TxnResponse.mk (default_val _) (default_val _) (default_val _) (default_val _) (default_val _) (default_val _);
+  to_val_has_go_type := ltac:(destruct falso);
+  default_val_eq_zero_val := ltac:(destruct falso);
+  to_val_inj := ltac:(destruct falso);
+  to_val_eqdec := ltac:(solve_decision);
+|}.
+Global Instance into_val_struct_field_TxnResponse_Header `{ffi_syntax} : IntoValStructField "Header" etcdserverpb.TxnResponse TxnResponse.Header'.
+Admitted.
+
+Global Instance into_val_struct_field_TxnResponse_Succeeded `{ffi_syntax} : IntoValStructField "Succeeded" etcdserverpb.TxnResponse TxnResponse.Succeeded'.
+Admitted.
+
+Global Instance into_val_struct_field_TxnResponse_Responses `{ffi_syntax} : IntoValStructField "Responses" etcdserverpb.TxnResponse TxnResponse.Responses'.
+Admitted.
+
+Global Instance into_val_struct_field_TxnResponse_XXX_NoUnkeyedLiteral `{ffi_syntax} : IntoValStructField "XXX_NoUnkeyedLiteral" etcdserverpb.TxnResponse TxnResponse.XXX_NoUnkeyedLiteral'.
+Admitted.
+
+Global Instance into_val_struct_field_TxnResponse_XXX_unrecognized `{ffi_syntax} : IntoValStructField "XXX_unrecognized" etcdserverpb.TxnResponse TxnResponse.XXX_unrecognized'.
+Admitted.
+
+Global Instance into_val_struct_field_TxnResponse_XXX_sizecache `{ffi_syntax} : IntoValStructField "XXX_sizecache" etcdserverpb.TxnResponse TxnResponse.XXX_sizecache'.
+Admitted.
+
+Instance wp_struct_make_TxnResponse `{ffi_semantics} `{!ffi_interp ffi} `{!heapGS Σ} Header' Succeeded' Responses' XXX_NoUnkeyedLiteral' XXX_unrecognized' XXX_sizecache':
+  PureWp True
+    (struct.make etcdserverpb.TxnResponse (alist_val [
+      "Header" ::= #Header';
+      "Succeeded" ::= #Succeeded';
+      "Responses" ::= #Responses';
+      "XXX_NoUnkeyedLiteral" ::= #XXX_NoUnkeyedLiteral';
+      "XXX_unrecognized" ::= #XXX_unrecognized';
+      "XXX_sizecache" ::= #XXX_sizecache'
+    ]))%V
+    #(TxnResponse.mk Header' Succeeded' Responses' XXX_NoUnkeyedLiteral' XXX_unrecognized' XXX_sizecache').
+Admitted.
+
 (* autogenerated by proofgen (names); do not modify *)
 Require Import New.code.go_etcd_io.etcd.api.v3.etcdserverpb.
 Require Export New.proof.proof_prelude.
