new/generatedproof/go_etcd_io/raft/v3/raftpb.v
@@ -4,6 +4,36 @@ From New.golang Require Import theory.
 
 Axiom falso : False.
 
+Module ConfChangeI.
+Section def.
+Context `{ffi_syntax}.
+Definition t := interface.t.
+End def.
+End ConfChangeI.
+Module EntryType.
+Section def.
+Context `{ffi_syntax}.
+Definition t := w32.
+End def.
+End EntryType.
+Module MessageType.
+Section def.
+Context `{ffi_syntax}.
+Definition t := w32.
+End def.
+End MessageType.
+Module ConfChangeTransition.
+Section def.
+Context `{ffi_syntax}.
+Definition t := w32.
+End def.
+End ConfChangeTransition.
+Module ConfChangeType.
+Section def.
+Context `{ffi_syntax}.
+Definition t := w32.
+End def.
+End ConfChangeType.
 Module Entry.
 Section def.
 Context `{ffi_syntax}.
@@ -193,102 +223,15 @@ Admitted.
 Module Message.
 Section def.
 Context `{ffi_syntax}.
-Record t := mk {
-  Type' : w32;
-  To' : w64;
-  From' : w64;
-  Term' : w64;
-  LogTerm' : w64;
-  Index' : w64;
-  Entries' : slice.t;
-  Commit' : w64;
-  Vote' : w64;
-  Snapshot' : loc;
-  Reject' : bool;
-  RejectHint' : w64;
-  Context' : slice.t;
-  Responses' : slice.t;
-}.
+Axiom t : Type.
 End def.
 End Message.
 
-
-Global Instance settable_Message `{ffi_syntax}: Settable _ :=
-  settable! Message.mk < Message.Type'; Message.To'; Message.From'; Message.Term'; Message.LogTerm'; Message.Index'; Message.Entries'; Message.Commit'; Message.Vote'; Message.Snapshot'; Message.Reject'; Message.RejectHint'; Message.Context'; Message.Responses' >.
 Global Instance into_val_Message `{ffi_syntax} : IntoVal Message.t.
 Admitted.
 
-Global Instance into_val_typed_Message `{ffi_syntax} : IntoValTyped Message.t raftpb.Message :=
-{|
-  default_val := Message.mk (default_val _) (default_val _) (default_val _) (default_val _) (default_val _) (default_val _) (default_val _) (default_val _) (default_val _) (default_val _) (default_val _) (default_val _) (default_val _) (default_val _);
-  to_val_has_go_type := ltac:(destruct falso);
-  default_val_eq_zero_val := ltac:(destruct falso);
-  to_val_inj := ltac:(destruct falso);
-  to_val_eqdec := ltac:(solve_decision);
-|}.
-Global Instance into_val_struct_field_Message_Type `{ffi_syntax} : IntoValStructField "Type" raftpb.Message Message.Type'.
+Global Instance into_val_typed_Message `{ffi_syntax} : IntoValTyped Message.t raftpb.Message.
 Admitted.
-
-Global Instance into_val_struct_field_Message_To `{ffi_syntax} : IntoValStructField "To" raftpb.Message Message.To'.
-Admitted.
-
-Global Instance into_val_struct_field_Message_From `{ffi_syntax} : IntoValStructField "From" raftpb.Message Message.From'.
-Admitted.
-
-Global Instance into_val_struct_field_Message_Term `{ffi_syntax} : IntoValStructField "Term" raftpb.Message Message.Term'.
-Admitted.
-
-Global Instance into_val_struct_field_Message_LogTerm `{ffi_syntax} : IntoValStructField "LogTerm" raftpb.Message Message.LogTerm'.
-Admitted.
-
-Global Instance into_val_struct_field_Message_Index `{ffi_syntax} : IntoValStructField "Index" raftpb.Message Message.Index'.
-Admitted.
-
-Global Instance into_val_struct_field_Message_Entries `{ffi_syntax} : IntoValStructField "Entries" raftpb.Message Message.Entries'.
-Admitted.
-
-Global Instance into_val_struct_field_Message_Commit `{ffi_syntax} : IntoValStructField "Commit" raftpb.Message Message.Commit'.
-Admitted.
-
-Global Instance into_val_struct_field_Message_Vote `{ffi_syntax} : IntoValStructField "Vote" raftpb.Message Message.Vote'.
-Admitted.
-
-Global Instance into_val_struct_field_Message_Snapshot `{ffi_syntax} : IntoValStructField "Snapshot" raftpb.Message Message.Snapshot'.
-Admitted.
-
-Global Instance into_val_struct_field_Message_Reject `{ffi_syntax} : IntoValStructField "Reject" raftpb.Message Message.Reject'.
-Admitted.
-
-Global Instance into_val_struct_field_Message_RejectHint `{ffi_syntax} : IntoValStructField "RejectHint" raftpb.Message Message.RejectHint'.
-Admitted.
-
-Global Instance into_val_struct_field_Message_Context `{ffi_syntax} : IntoValStructField "Context" raftpb.Message Message.Context'.
-Admitted.
-
-Global Instance into_val_struct_field_Message_Responses `{ffi_syntax} : IntoValStructField "Responses" raftpb.Message Message.Responses'.
-Admitted.
-
-Instance wp_struct_make_Message `{ffi_semantics} `{!ffi_interp ffi} `{!heapGS Σ} Type' To' From' Term' LogTerm' Index' Entries' Commit' Vote' Snapshot' Reject' RejectHint' Context' Responses':
-  PureWp True
-    (struct.make raftpb.Message (alist_val [
-      "Type" ::= #Type';
-      "To" ::= #To';
-      "From" ::= #From';
-      "Term" ::= #Term';
-      "LogTerm" ::= #LogTerm';
-      "Index" ::= #Index';
-      "Entries" ::= #Entries';
-      "Commit" ::= #Commit';
-      "Vote" ::= #Vote';
-      "Snapshot" ::= #Snapshot';
-      "Reject" ::= #Reject';
-      "RejectHint" ::= #RejectHint';
-      "Context" ::= #Context';
-      "Responses" ::= #Responses'
-    ]))%V
-    #(Message.mk Type' To' From' Term' LogTerm' Index' Entries' Commit' Vote' Snapshot' Reject' RejectHint' Context' Responses').
-Admitted.
-
 Module HardState.
 Section def.
 Context `{ffi_syntax}.
